@prefix : <http://www.w3.org/2003/06/sw-vocab-status/ns#> .
@prefix v: <http://rdf.data-vocabulary.org/#> .
@prefix dc: <http://purl.org/dc/elements/1.1/> .
@prefix fo: <http://purl.org/ontology/fo/> .
@prefix vs: <http://www.w3.org/2003/06/sw-vocab-status/ns#> .
@prefix owl: <http://www.w3.org/2002/07/owl#> .
@prefix rdf: <http://www.w3.org/1999/02/22-rdf-syntax-ns#> .
@prefix xml: <http://www.w3.org/XML/1998/namespace> .
@prefix xsd: <http://www.w3.org/2001/XMLSchema#> .
@prefix foaf: <http://xmlns.com/foaf/0.1/> .
@prefix rdfs: <http://www.w3.org/2000/01/rdf-schema#> .
@prefix skos: <http://www.w3.org/2004/02/skos/core#> .
@prefix dcmit: <http://purl.org/dc/dcmitype/> .
@prefix dcterms: <http://purl.org/dc/terms/> .
@prefix dctypes: <http://purl.org/dc/dcmitype/> .
@prefix provenance: <http://www.bbc.co.uk/ontologies/provenance/> .
@base <http://www.w3.org/2003/06/sw-vocab-status/ns#> .

<http://www.w3.org/2003/06/sw-vocab-status/ns#> rdf:type owl:Ontology ;
                                                 owl:versionIRI fo: ;
                                                 owl:imports <http://www.w3.org/2003/06/sw-vocab-status/ns#> ,
                                                             provenance: ,
                                                             foaf: ;
                                                 provenance:public "true"^^xsd:boolean ;
                                                 provenance:canonicalLocation "https://repo.dev.bbc.co.uk/services/linked-data/ontologies/domain/kl/food/food-ontology-1-1.ttl"^^xsd:string ;
                                                 provenance:changeReason "Fix a typo of occassion"^^xsd:string ;
                                                 owl:priorVersion fo: ;
                                                 provenance:version "1.1"^^xsd:double ;
                                                 owl:versionInfo "1.1"^^xsd:string ;
                                                 dcterms:license <http://creativecommons.org/licenses/by/4.0#id> ;
                                                 dcterms:created "2011-07-08"^^xsd:date ;
                                                 dcterms:title "Food Ontology"@en-gb ;
                                                 provenance:slug "fo"^^xsd:string ;
                                                 rdfs:comment "A simple vocabulary for describing recipes, ingredients, menus and diets."@en-gb ;
                                                 rdfs:label "Food Ontology"^^xsd:string ;
                                                 dc:date "Date: 2014/03/18 16:30:00 " .

#################################################################
#    Annotation properties
#################################################################

###  http://purl.org/dc/elements/1.1/contributor
dc:contributor rdf:type owl:AnnotationProperty ;
               dcterms:description "Examples of a Contributor include a person, an organization, or a service. Typically, the name of a Contributor should be used to indicate the entity."@en ;
               dcterms:hasVersion <http://dublincore.org/usage/terms/history/#contributor-006> ;
               dcterms:issued "1999-07-02"^^xsd:date ;
               dcterms:modified "2008-01-14"^^xsd:date ;
               rdfs:comment "An entity responsible for making contributions to the resource."@en ;
               rdfs:isDefinedBy dc: ;
               rdfs:label "Contributor"@en ;
               skos:note "A second property with the same name as this property has been declared in the dcterms: namespace (http://purl.org/dc/terms/).  See the Introduction to the document \"DCMI Metadata Terms\" (http://dublincore.org/documents/dcmi-terms/) for an explanation."@en .


###  http://purl.org/dc/elements/1.1/coverage
dc:coverage rdf:type owl:AnnotationProperty ;
            dcterms:description "Spatial topic and spatial applicability may be a named place or a location specified by its geographic coordinates. Temporal topic may be a named period, date, or date range. A jurisdiction may be a named administrative entity or a geographic place to which the resource applies. Recommended best practice is to use a controlled vocabulary such as the Thesaurus of Geographic Names [TGN]. Where appropriate, named places or time periods can be used in preference to numeric identifiers such as sets of coordinates or date ranges."@en ;
            dcterms:hasVersion <http://dublincore.org/usage/terms/history/#coverage-006> ;
            dcterms:issued "1999-07-02"^^xsd:date ;
            dcterms:modified "2008-01-14"^^xsd:date ;
            rdfs:comment "The spatial or temporal topic of the resource, the spatial applicability of the resource, or the jurisdiction under which the resource is relevant."@en ;
            rdfs:isDefinedBy dc: ;
            rdfs:label "Coverage"@en ;
            skos:note "A second property with the same name as this property has been declared in the dcterms: namespace (http://purl.org/dc/terms/).  See the Introduction to the document \"DCMI Metadata Terms\" (http://dublincore.org/documents/dcmi-terms/) for an explanation."@en .


###  http://purl.org/dc/elements/1.1/creator
dc:creator rdf:type owl:AnnotationProperty ;
           dcterms:description "Examples of a Creator include a person, an organization, or a service. Typically, the name of a Creator should be used to indicate the entity."@en ;
           dcterms:hasVersion <http://dublincore.org/usage/terms/history/#creator-006> ;
           dcterms:issued "1999-07-02"^^xsd:date ;
           dcterms:modified "2008-01-14"^^xsd:date ;
           rdfs:comment "An entity primarily responsible for making the resource."@en ;
           rdfs:isDefinedBy dc: ;
           rdfs:label "Creator"@en ;
           skos:note "A second property with the same name as this property has been declared in the dcterms: namespace (http://purl.org/dc/terms/).  See the Introduction to the document \"DCMI Metadata Terms\" (http://dublincore.org/documents/dcmi-terms/) for an explanation."@en .


###  http://purl.org/dc/elements/1.1/date
dc:date dcterms:description "Date may be used to express temporal information at any level of granularity.  Recommended best practice is to use an encoding scheme, such as the W3CDTF profile of ISO 8601 [W3CDTF]."@en ;
        dcterms:hasVersion <http://dublincore.org/usage/terms/history/#date-006> ;
        dcterms:issued "1999-07-02"^^xsd:date ;
        dcterms:modified "2008-01-14"^^xsd:date ;
        rdfs:comment "A point or period of time associated with an event in the lifecycle of the resource."@en ;
        rdfs:isDefinedBy dc: ;
        rdfs:label "Date"@en ;
        skos:note "A second property with the same name as this property has been declared in the dcterms: namespace (http://purl.org/dc/terms/).  See the Introduction to the document \"DCMI Metadata Terms\" (http://dublincore.org/documents/dcmi-terms/) for an explanation."@en .


###  http://purl.org/dc/elements/1.1/description
dc:description dcterms:description "Description may include but is not limited to: an abstract, a table of contents, a graphical representation, or a free-text account of the resource."@en ;
               dcterms:hasVersion <http://dublincore.org/usage/terms/history/#description-006> ;
               dcterms:issued "1999-07-02"^^xsd:date ;
               dcterms:modified "2008-01-14"^^xsd:date ;
               rdfs:comment "An account of the resource."@en ;
               rdfs:isDefinedBy dc: ;
               rdfs:label "Description"@en ;
               skos:note "A second property with the same name as this property has been declared in the dcterms: namespace (http://purl.org/dc/terms/).  See the Introduction to the document \"DCMI Metadata Terms\" (http://dublincore.org/documents/dcmi-terms/) for an explanation."@en .


###  http://purl.org/dc/elements/1.1/format
dc:format rdf:type owl:AnnotationProperty ;
          dcterms:description "Examples of dimensions include size and duration. Recommended best practice is to use a controlled vocabulary such as the list of Internet Media Types [MIME]."@en ;
          dcterms:hasVersion <http://dublincore.org/usage/terms/history/#format-007> ;
          dcterms:issued "1999-07-02"^^xsd:date ;
          dcterms:modified "2008-01-14"^^xsd:date ;
          rdfs:comment "The file format, physical medium, or dimensions of the resource."@en ;
          rdfs:isDefinedBy dc: ;
          rdfs:label "Format"@en ;
          skos:note "A second property with the same name as this property has been declared in the dcterms: namespace (http://purl.org/dc/terms/).  See the Introduction to the document \"DCMI Metadata Terms\" (http://dublincore.org/documents/dcmi-terms/) for an explanation."@en .


###  http://purl.org/dc/elements/1.1/identifier
dc:identifier rdf:type owl:AnnotationProperty ;
              dcterms:description "Recommended best practice is to identify the resource by means of a string conforming to a formal identification system. "@en ;
              dcterms:hasVersion <http://dublincore.org/usage/terms/history/#identifier-006> ;
              dcterms:issued "1999-07-02"^^xsd:date ;
              dcterms:modified "2008-01-14"^^xsd:date ;
              rdfs:comment "An unambiguous reference to the resource within a given context."@en ;
              rdfs:isDefinedBy dc: ;
              rdfs:label "Identifier"@en ;
              skos:note "A second property with the same name as this property has been declared in the dcterms: namespace (http://purl.org/dc/terms/).  See the Introduction to the document \"DCMI Metadata Terms\" (http://dublincore.org/documents/dcmi-terms/) for an explanation."@en .


###  http://purl.org/dc/elements/1.1/language
dc:language rdf:type owl:AnnotationProperty ;
            dcterms:description "Recommended best practice is to use a controlled vocabulary such as RFC 4646 [RFC4646]."@en ;
            dcterms:hasVersion <http://dublincore.org/usage/terms/history/#language-007> ;
            dcterms:issued "1999-07-02"^^xsd:date ;
            dcterms:modified "2008-01-14"^^xsd:date ;
            rdfs:comment "A language of the resource."@en ;
            rdfs:isDefinedBy dc: ;
            rdfs:label "Language"@en ;
            rdfs:seeAlso <http://www.ietf.org/rfc/rfc4646.txt> ;
            skos:note "A second property with the same name as this property has been declared in the dcterms: namespace (http://purl.org/dc/terms/).  See the Introduction to the document \"DCMI Metadata Terms\" (http://dublincore.org/documents/dcmi-terms/) for an explanation."@en .


###  http://purl.org/dc/elements/1.1/publisher
dc:publisher rdf:type owl:AnnotationProperty ;
             dcterms:description "Examples of a Publisher include a person, an organization, or a service. Typically, the name of a Publisher should be used to indicate the entity."@en ;
             dcterms:hasVersion <http://dublincore.org/usage/terms/history/#publisher-006> ;
             dcterms:issued "1999-07-02"^^xsd:date ;
             dcterms:modified "2008-01-14"^^xsd:date ;
             rdfs:comment "An entity responsible for making the resource available."@en ;
             rdfs:isDefinedBy dc: ;
             rdfs:label "Publisher"@en ;
             skos:note "A second property with the same name as this property has been declared in the dcterms: namespace (http://purl.org/dc/terms/).  See the Introduction to the document \"DCMI Metadata Terms\" (http://dublincore.org/documents/dcmi-terms/) for an explanation."@en .


###  http://purl.org/dc/elements/1.1/relation
dc:relation rdf:type owl:AnnotationProperty ;
            dcterms:description "Recommended best practice is to identify the related resource by means of a string conforming to a formal identification system. "@en ;
            dcterms:hasVersion <http://dublincore.org/usage/terms/history/#relation-006> ;
            dcterms:issued "1999-07-02"^^xsd:date ;
            dcterms:modified "2008-01-14"^^xsd:date ;
            rdfs:comment "A related resource."@en ;
            rdfs:isDefinedBy dc: ;
            rdfs:label "Relation"@en ;
            skos:note "A second property with the same name as this property has been declared in the dcterms: namespace (http://purl.org/dc/terms/).  See the Introduction to the document \"DCMI Metadata Terms\" (http://dublincore.org/documents/dcmi-terms/) for an explanation."@en .


###  http://purl.org/dc/elements/1.1/rights
dc:rights rdf:type owl:AnnotationProperty ;
          dcterms:description "Typically, rights information includes a statement about various property rights associated with the resource, including intellectual property rights."@en ;
          dcterms:hasVersion <http://dublincore.org/usage/terms/history/#rights-006> ;
          dcterms:issued "1999-07-02"^^xsd:date ;
          dcterms:modified "2008-01-14"^^xsd:date ;
          rdfs:comment "Information about rights held in and over the resource."@en ;
          rdfs:isDefinedBy dc: ;
          rdfs:label "Rights"@en ;
          skos:note "A second property with the same name as this property has been declared in the dcterms: namespace (http://purl.org/dc/terms/).  See the Introduction to the document \"DCMI Metadata Terms\" (http://dublincore.org/documents/dcmi-terms/) for an explanation."@en .


###  http://purl.org/dc/elements/1.1/source
dc:source rdf:type owl:AnnotationProperty ;
          dcterms:description "The described resource may be derived from the related resource in whole or in part. Recommended best practice is to identify the related resource by means of a string conforming to a formal identification system."@en ;
          dcterms:hasVersion <http://dublincore.org/usage/terms/history/#source-006> ;
          dcterms:issued "1999-07-02"^^xsd:date ;
          dcterms:modified "2008-01-14"^^xsd:date ;
          rdfs:comment "A related resource from which the described resource is derived."@en ;
          rdfs:isDefinedBy dc: ;
          rdfs:label "Source"@en ;
          skos:note "A second property with the same name as this property has been declared in the dcterms: namespace (http://purl.org/dc/terms/).  See the Introduction to the document \"DCMI Metadata Terms\" (http://dublincore.org/documents/dcmi-terms/) for an explanation."@en .


###  http://purl.org/dc/elements/1.1/subject
dc:subject rdf:type owl:AnnotationProperty ;
           dcterms:description "Typically, the subject will be represented using keywords, key phrases, or classification codes. Recommended best practice is to use a controlled vocabulary."@en ;
           dcterms:hasVersion <http://dublincore.org/usage/terms/history/#subject-007> ;
           dcterms:issued "1999-07-02"^^xsd:date ;
           dcterms:modified "2012-06-14"^^xsd:date ;
           rdfs:comment "The topic of the resource."@en ;
           rdfs:isDefinedBy dc: ;
           rdfs:label "Subject"@en ;
           skos:note "A second property with the same name as this property has been declared in the dcterms: namespace (http://purl.org/dc/terms/).  See the Introduction to the document \"DCMI Metadata Terms\" (http://dublincore.org/documents/dcmi-terms/) for an explanation."@en .


###  http://purl.org/dc/elements/1.1/title
dc:title dcterms:hasVersion <http://dublincore.org/usage/terms/history/#title-006> ;
         dcterms:issued "1999-07-02"^^xsd:date ;
         dcterms:modified "2008-01-14"^^xsd:date ;
         rdfs:comment "A name given to the resource."@en ;
         rdfs:isDefinedBy dc: ;
         rdfs:label "Title"@en ;
         skos:note "A second property with the same name as this property has been declared in the dcterms: namespace (http://purl.org/dc/terms/).  See the Introduction to the document \"DCMI Metadata Terms\" (http://dublincore.org/documents/dcmi-terms/) for an explanation."@en .


###  http://purl.org/dc/elements/1.1/type
dc:type rdf:type owl:AnnotationProperty ;
        dcterms:description "Recommended best practice is to use a controlled vocabulary such as the DCMI Type Vocabulary [DCMITYPE]. To describe the file format, physical medium, or dimensions of the resource, use the Format element."@en ;
        dcterms:hasVersion <http://dublincore.org/usage/terms/history/#type-006> ;
        dcterms:issued "1999-07-02"^^xsd:date ;
        dcterms:modified "2008-01-14"^^xsd:date ;
        rdfs:comment "The nature or genre of the resource."@en ;
        rdfs:isDefinedBy dc: ;
        rdfs:label "Type"@en ;
        skos:note "A second property with the same name as this property has been declared in the dcterms: namespace (http://purl.org/dc/terms/).  See the Introduction to the document \"DCMI Metadata Terms\" (http://dublincore.org/documents/dcmi-terms/) for an explanation."@en .


###  http://purl.org/dc/terms/abstract
dcterms:abstract rdf:type owl:AnnotationProperty ;
                 rdfs:subPropertyOf dc:description ,
                                    dcterms:description .


###  http://purl.org/dc/terms/accessRights
dcterms:accessRights rdf:type owl:AnnotationProperty ;
                     rdfs:subPropertyOf dc:rights ,
                                        dcterms:rights .


###  http://purl.org/dc/terms/alternative
dcterms:alternative rdf:type owl:AnnotationProperty ;
                    rdfs:subPropertyOf dc:title ;
                    rdfs:range rdfs:Literal .


###  http://purl.org/dc/terms/available
dcterms:available rdf:type owl:AnnotationProperty ;
                  rdfs:subPropertyOf dc:date ;
                  rdfs:range rdfs:Literal .


###  http://purl.org/dc/terms/bibliographicCitation
dcterms:bibliographicCitation rdf:type owl:AnnotationProperty ;
                              rdfs:subPropertyOf dc:identifier ;
                              rdfs:range rdfs:Literal .


###  http://purl.org/dc/terms/conformsTo
dcterms:conformsTo rdf:type owl:AnnotationProperty ;
                   rdfs:subPropertyOf dc:relation ,
                                      dcterms:relation .


###  http://purl.org/dc/terms/contributor
dcterms:contributor rdf:type owl:AnnotationProperty ;
                    rdfs:subPropertyOf dc:contributor .


###  http://purl.org/dc/terms/coverage
dcterms:coverage rdf:type owl:AnnotationProperty ;
                 rdfs:subPropertyOf dc:coverage .


###  http://purl.org/dc/terms/created
dcterms:created rdf:type owl:AnnotationProperty ;
                rdfs:subPropertyOf dc:date ;
                rdfs:range rdfs:Literal .


###  http://purl.org/dc/terms/creator
dcterms:creator rdf:type owl:AnnotationProperty ;
                rdfs:subPropertyOf dc:creator ,
                                   dcterms:contributor .


###  http://purl.org/dc/terms/date
dcterms:date rdf:type owl:AnnotationProperty ;
             rdfs:subPropertyOf dc:date ;
             rdfs:range rdfs:Literal .


###  http://purl.org/dc/terms/dateAccepted
dcterms:dateAccepted rdf:type owl:AnnotationProperty ;
                     rdfs:subPropertyOf dc:date ;
                     rdfs:range rdfs:Literal .


###  http://purl.org/dc/terms/dateCopyrighted
dcterms:dateCopyrighted rdf:type owl:AnnotationProperty ;
                        rdfs:subPropertyOf dc:date ;
                        rdfs:range rdfs:Literal .


###  http://purl.org/dc/terms/dateSubmitted
dcterms:dateSubmitted rdf:type owl:AnnotationProperty ;
                      rdfs:subPropertyOf dc:date ;
                      rdfs:range rdfs:Literal .


###  http://purl.org/dc/terms/description
dcterms:description rdf:type owl:AnnotationProperty ;
                    rdfs:subPropertyOf dc:description .


###  http://purl.org/dc/terms/extent
dcterms:extent rdf:type owl:AnnotationProperty ;
               rdfs:subPropertyOf dc:format ,
                                  dcterms:format .


###  http://purl.org/dc/terms/format
dcterms:format rdf:type owl:AnnotationProperty ;
               rdfs:subPropertyOf dc:format .


###  http://purl.org/dc/terms/hasFormat
dcterms:hasFormat rdf:type owl:AnnotationProperty ;
                  rdfs:subPropertyOf dc:relation ,
                                     dcterms:relation .


###  http://purl.org/dc/terms/hasPart
dcterms:hasPart rdf:type owl:AnnotationProperty ;
                rdfs:subPropertyOf dc:relation ,
                                   dcterms:relation .


###  http://purl.org/dc/terms/hasVersion
dcterms:hasVersion rdf:type owl:AnnotationProperty ;
                   rdfs:subPropertyOf dc:relation ,
                                      dcterms:relation .


###  http://purl.org/dc/terms/identifier
dcterms:identifier rdf:type owl:AnnotationProperty ;
                   rdfs:subPropertyOf dc:identifier ;
                   rdfs:range rdfs:Literal .


###  http://purl.org/dc/terms/isFormatOf
dcterms:isFormatOf rdf:type owl:AnnotationProperty ;
                   rdfs:subPropertyOf dc:relation ,
                                      dcterms:relation .


###  http://purl.org/dc/terms/isPartOf
dcterms:isPartOf rdf:type owl:AnnotationProperty ;
                 rdfs:subPropertyOf dc:relation ,
                                    dcterms:relation .


###  http://purl.org/dc/terms/isReferencedBy
dcterms:isReferencedBy rdf:type owl:AnnotationProperty ;
                       rdfs:subPropertyOf dc:relation ,
                                          dcterms:relation .


###  http://purl.org/dc/terms/isReplacedBy
dcterms:isReplacedBy rdf:type owl:AnnotationProperty ;
                     rdfs:subPropertyOf dc:relation ,
                                        dcterms:relation .


###  http://purl.org/dc/terms/isRequiredBy
dcterms:isRequiredBy rdf:type owl:AnnotationProperty ;
                     rdfs:subPropertyOf dc:relation ,
                                        dcterms:relation .


###  http://purl.org/dc/terms/isVersionOf
dcterms:isVersionOf rdf:type owl:AnnotationProperty ;
                    rdfs:subPropertyOf dc:relation ,
                                       dcterms:relation .


###  http://purl.org/dc/terms/issued
dcterms:issued rdf:type owl:AnnotationProperty ;
               rdfs:subPropertyOf dc:date ;
               rdfs:range rdfs:Literal .


###  http://purl.org/dc/terms/language
dcterms:language rdf:type owl:AnnotationProperty ;
                 rdfs:subPropertyOf dc:language .


###  http://purl.org/dc/terms/license
dcterms:license rdf:type owl:AnnotationProperty ;
                rdfs:subPropertyOf dc:rights ,
                                   dcterms:rights .


###  http://purl.org/dc/terms/medium
dcterms:medium rdf:type owl:AnnotationProperty ;
               rdfs:subPropertyOf dc:format ,
                                  dcterms:format .


###  http://purl.org/dc/terms/modified
dcterms:modified rdf:type owl:AnnotationProperty ;
                 rdfs:subPropertyOf dc:date ;
                 rdfs:range rdfs:Literal .


###  http://purl.org/dc/terms/publisher
dcterms:publisher rdf:type owl:AnnotationProperty ;
                  rdfs:subPropertyOf dc:publisher .


###  http://purl.org/dc/terms/references
dcterms:references rdf:type owl:AnnotationProperty ;
                   rdfs:subPropertyOf dc:relation ,
                                      dcterms:relation .


###  http://purl.org/dc/terms/relation
dcterms:relation rdf:type owl:AnnotationProperty ;
                 rdfs:subPropertyOf dc:relation .


###  http://purl.org/dc/terms/replaces
dcterms:replaces rdf:type owl:AnnotationProperty ;
                 rdfs:subPropertyOf dc:relation ,
                                    dcterms:relation .


###  http://purl.org/dc/terms/requires
dcterms:requires rdf:type owl:AnnotationProperty ;
                 rdfs:subPropertyOf dc:relation ,
                                    dcterms:relation .


###  http://purl.org/dc/terms/rights
dcterms:rights rdf:type owl:AnnotationProperty ;
               rdfs:subPropertyOf dc:rights .


###  http://purl.org/dc/terms/source
dcterms:source rdf:type owl:AnnotationProperty ;
               rdfs:subPropertyOf dc:source ,
                                  dcterms:relation .


###  http://purl.org/dc/terms/spatial
dcterms:spatial rdf:type owl:AnnotationProperty ;
                rdfs:subPropertyOf dc:coverage ,
                                   dcterms:coverage .


###  http://purl.org/dc/terms/subject
dcterms:subject rdf:type owl:AnnotationProperty ;
                rdfs:subPropertyOf dc:subject .


###  http://purl.org/dc/terms/tableOfContents
dcterms:tableOfContents rdf:type owl:AnnotationProperty ;
                        rdfs:subPropertyOf dc:description ,
                                           dcterms:description .


###  http://purl.org/dc/terms/temporal
dcterms:temporal rdf:type owl:AnnotationProperty ;
                 rdfs:subPropertyOf dc:coverage ,
                                    dcterms:coverage .


###  http://purl.org/dc/terms/title
dcterms:title rdf:type owl:AnnotationProperty ;
              rdfs:subPropertyOf dc:title ;
              rdfs:range rdfs:Literal .


###  http://purl.org/dc/terms/type
dcterms:type rdf:type owl:AnnotationProperty ;
             rdfs:subPropertyOf dc:type .


###  http://purl.org/dc/terms/valid
dcterms:valid rdf:type owl:AnnotationProperty ;
              rdfs:subPropertyOf dc:date ;
              rdfs:range rdfs:Literal .


###  http://www.w3.org/2004/02/skos/core#note
skos:note rdf:type owl:AnnotationProperty .


#################################################################
#    Datatypes
#################################################################

###  http://www.w3.org/2001/XMLSchema#date
xsd:date rdf:type rdfs:Datatype .


#################################################################
#    Object Properties
#################################################################

###  http://purl.org/ontology/fo/at_its_best
fo:at_its_best rdf:type owl:ObjectProperty ;
               rdfs:domain fo:Food ;
               rdfs:range fo:Season ;
               rdfs:comment "The at its best property tells us in what season a particular food is at its best."@en-gb ;
               rdfs:isDefinedBy fo: ;
               rdfs:label "at its best"@en-gb ;
               vs:term_status "testing" .


###  http://purl.org/ontology/fo/canape
fo:canape rdf:type owl:ObjectProperty ;
          rdfs:range fo:Recipe ;
          rdfs:comment "The canape property relates a menu to a recipe that may be served as a canape."@en-gb ;
          rdfs:isDefinedBy fo: ;
          rdfs:label "canape"@en-gb ;
          vs:term_status "testing" .


###  http://purl.org/ontology/fo/cuisine
fo:cuisine rdf:type owl:ObjectProperty ;
           rdfs:domain fo:Recipe ;
           rdfs:range fo:Cuisine ;
           rdfs:comment "The cuisine property classifies a recipe as being an example of that cuisine."@en-gb ;
           rdfs:isDefinedBy fo: ;
           rdfs:label "cuisine"@en-gb ;
           vs:term_status "testing" .


###  http://purl.org/ontology/fo/dessert
fo:dessert rdf:type owl:ObjectProperty ;
           rdfs:range fo:Recipe ;
           rdfs:comment "The dessert property relates a menu to a recipe that may be served as a dessert."@en-gb ;
           rdfs:isDefinedBy fo: ;
           rdfs:label "dessert"@en-gb ;
           vs:term_status "testing" .


###  http://purl.org/ontology/fo/diet
fo:diet rdf:type owl:ObjectProperty ;
        rdfs:domain fo:Recipe ;
        rdfs:comment "The diet property relates a recipe to a diet it may be suitable for."@en-gb ;
        rdfs:isDefinedBy fo: ;
        rdfs:label "diet"@en-gb ;
        vs:term_status "testing" .


###  http://purl.org/ontology/fo/food
fo:food rdf:type owl:ObjectProperty ;
        rdfs:domain fo:Ingredient ;
        rdfs:range fo:Food ;
        rdfs:comment "The food property relates an ingredient to the food that is required."@en-gb ;
        rdfs:isDefinedBy fo: ;
        rdfs:label "food"@en-gb ;
        vs:term_status "testing" .


###  http://purl.org/ontology/fo/ingredients
fo:ingredients rdf:type owl:ObjectProperty ;
               rdfs:range fo:IngredientList ;
               rdfs:comment "The ingredients property relates a recipe or recipe stage to an ingredient list."@en-gb ;
               rdfs:isDefinedBy fo: ;
               rdfs:label "ingredients"@en-gb ;
               vs:term_status "testing" .


###  http://purl.org/ontology/fo/main_course
fo:main_course rdf:type owl:ObjectProperty ;
               rdfs:range fo:Recipe ;
               rdfs:comment "The main course property relates a menu to a recipe that may be served as a main course."@en-gb ;
               rdfs:isDefinedBy fo: ;
               rdfs:label "main course"@en-gb ;
               vs:term_status "testing" .


###  http://purl.org/ontology/fo/method
fo:method rdf:type owl:ObjectProperty ;
          rdfs:range fo:Method ;
          rdfs:comment "The method property relates a recipe or stage to the method used to make it."@en-gb ;
          rdfs:isDefinedBy fo: ;
          rdfs:label "method"@en-gb ;
          vs:term_status "testing" .


###  http://purl.org/ontology/fo/occasion
fo:occasion rdf:type owl:ObjectProperty ;
            rdfs:domain fo:Recipe ;
            rdfs:range fo:Occasion ;
            rdfs:comment "The occassion property relates a recipe to an occasion it may be appropriate for."@en-gb ;
            rdfs:isDefinedBy fo: ;
            rdfs:label "occassion"@en-gb ;
            vs:term_status "testing" .


###  http://purl.org/ontology/fo/produces
fo:produces rdf:type owl:ObjectProperty ;
            rdfs:domain fo:Recipe ;
            rdfs:range fo:Food ;
            rdfs:comment "The produces property relates a recipe to the food it produces."@en-gb ;
            rdfs:isDefinedBy fo: ;
            rdfs:label "produces"@en-gb ;
            vs:term_status "testing" .


###  http://purl.org/ontology/fo/required_technique
fo:required_technique rdf:type owl:ObjectProperty ;
                      rdfs:range fo:Technique ;
                      rdfs:comment "The required technique property indicates that a particular technique is required in order to complete a recipe, method or step."@en-gb ;
                      rdfs:isDefinedBy fo: ;
                      rdfs:label "required technique"@en-gb ;
                      vs:term_status "testing" .


###  http://purl.org/ontology/fo/serve_as
fo:serve_as rdf:type owl:ObjectProperty ;
            rdfs:domain fo:Recipe ;
            rdfs:range fo:Course ;
            rdfs:comment "The serve as property relates a recipe to the course in a meal that it may be served as."@en-gb ;
            rdfs:isDefinedBy fo: ;
            rdfs:label "serve as"@en-gb ;
            vs:term_status "testing" .


###  http://purl.org/ontology/fo/shopping_category
fo:shopping_category rdf:type owl:ObjectProperty ;
                     rdfs:domain fo:Food ;
                     rdfs:comment "The shopping category property relates a food to the shopping category where that food is likely to be found when shopping for it."@en-gb ;
                     rdfs:isDefinedBy fo: ;
                     rdfs:label "shopping category"@en-gb ;
                     vs:term_status "testing" .


###  http://purl.org/ontology/fo/side_dish
fo:side_dish rdf:type owl:ObjectProperty ;
             rdfs:range fo:Recipe ;
             rdfs:comment "The side dish property relates a menu to a recipe that may be served as a side dish."@en-gb ;
             rdfs:isDefinedBy fo: ;
             rdfs:label "side dish"@en-gb ;
             vs:term_status "testing" .


###  http://purl.org/ontology/fo/stages
fo:stages rdf:type owl:ObjectProperty ;
          rdfs:domain fo:Recipe ;
          rdfs:range fo:StageSequence ;
          rdfs:comment "The stages property relates a recipe to the sequence of stages it contains."@en-gb ;
          rdfs:isDefinedBy fo: ;
          rdfs:label "stages"@en-gb ;
          vs:term_status "testing" .


###  http://purl.org/ontology/fo/starter
fo:starter rdf:type owl:ObjectProperty ;
           rdfs:range fo:Recipe ;
           rdfs:comment "The starter property relates a menu to a recipe that may be served as a starter."@en-gb ;
           rdfs:isDefinedBy fo: ;
           rdfs:label "starter"@en-gb ;
           vs:term_status "testing" .


#################################################################
#    Data properties
#################################################################

###  http://purl.org/ontology/fo/imperial_quantity
fo:imperial_quantity rdf:type owl:DatatypeProperty ;
                     rdfs:domain fo:Ingredient ;
                     rdfs:range xsd:string ;
                     rdfs:comment "A metric quantity provides a value and imperial unit in a human readable string for use in measuring out an ingredient."@en-gb ;
                     rdfs:isDefinedBy fo: ;
                     rdfs:label "imperial quantity"@en-gb ;
                     vs:term_status "testing" .


###  http://purl.org/ontology/fo/instruction
fo:instruction rdf:type owl:DatatypeProperty ;
               rdfs:range xsd:string ;
               rdfs:comment "An instruction provides the human-readable text associated with a step in the method for a recipe."@en-gb ;
               rdfs:isDefinedBy fo: ;
               rdfs:label "instruction"@en-gb ;
               vs:term_status "testing" .


###  http://purl.org/ontology/fo/metric_quantity
fo:metric_quantity rdf:type owl:DatatypeProperty ;
                   rdfs:domain fo:Ingredient ;
                   rdfs:range xsd:string ;
                   rdfs:comment "A metric quantity provides a value and metric unit in a human readable string for use in measuring out an ingredient."@en-gb ;
                   rdfs:isDefinedBy fo: ;
                   rdfs:label "metric quantity"@en-gb ;
                   vs:term_status "testing" .


###  http://purl.org/ontology/fo/quantity
fo:quantity rdf:type owl:DatatypeProperty ;
            rdfs:domain fo:Ingredient ;
            rdfs:range xsd:nonNegativeInteger ;
            rdfs:comment "A quantity provides a non-negative integer quantity that can be used as a measure of the food stuff for the ingredient."@en-gb ;
            rdfs:isDefinedBy fo: ;
            rdfs:label "quantity"@en-gb ;
            vs:term_status "testing" .


###  http://purl.org/ontology/fo/serves
fo:serves rdf:type owl:DatatypeProperty ;
          rdfs:domain fo:Recipe ;
          rdfs:range xsd:string ;
          rdfs:comment "The server property indicates what the recipe is intended to serve, this is often a human readable integer range such as '6-8'."@en-gb ;
          rdfs:isDefinedBy fo: ;
          rdfs:label "serves"@en-gb ;
          vs:term_status "testing" .


#################################################################
#    Classes
#################################################################

###  http://purl.org/ontology/fo/Course
fo:Course rdf:type owl:Class ;
          rdfs:comment "A Course is the sequence of a dish within a meal. For example a basic dinner party may consists of Starter, Main and Dessert courses."@en-gb ;
          rdfs:isDefinedBy fo: ;
          rdfs:label "Course"@en-gb ;
          vs:term_status "testing" .


###  http://purl.org/ontology/fo/Cuisine
fo:Cuisine rdf:type owl:Class ;
           rdfs:comment "A Cuisine is a particular style of food, often based on a region. These classifications are often highly subjective."@en-gb ;
           rdfs:isDefinedBy fo: ;
           rdfs:label "Cuisine"@en-gb ;
           vs:term_status "testing" .


###  http://purl.org/ontology/fo/Food
fo:Food rdf:type owl:Class ;
        rdfs:comment "A Food is something that can be eaten. It may be a basic food such as salt or it may be the more complex result of another recipe, for example chicken stock. A recipe uses foods as part of ingredients and also produces foods to be eaten."@en-gb ;
        rdfs:isDefinedBy fo: ;
        rdfs:label "Food"@en-gb ;
        vs:term_status "testing" .


###  http://purl.org/ontology/fo/Ingredient
fo:Ingredient rdf:type owl:Class .


###  http://purl.org/ontology/fo/IngredientList
fo:IngredientList rdf:type owl:Class ;
                  rdfs:subClassOf rdf:Seq ;
                  rdfs:comment "An IngredientList is a sequence (rdf:Seq) of ingredients in the order they should be listed in the recipe."@en-gb ;
                  rdfs:isDefinedBy fo: ;
                  rdfs:label "IngredientList"@en-gb ;
                  vs:term_status "testing" .


###  http://purl.org/ontology/fo/Method
fo:Method rdf:type owl:Class ;
          rdfs:subClassOf rdf:Seq ;
          rdfs:comment "A Method is the way in which ingredients are combined, using particular techniques, in order to produce a food. A method is part of a recipe and is also an rdf:Seq."@en-gb ;
          rdfs:isDefinedBy fo: ;
          rdfs:label "Method"@en-gb ;
          vs:term_status "testing" .


###  http://purl.org/ontology/fo/Occasion
fo:Occasion rdf:type owl:Class ;
            rdfs:comment "An Occasion is a recognised event or type of event that a particular food may be suitable for. An exmaple of a particular occassion might be Chinese New Year, whereas a more general occassion might a birthday."@en-gb ;
            rdfs:isDefinedBy fo: ;
            rdfs:label "Occasion"@en-gb ;
            vs:term_status "testing" .


###  http://purl.org/ontology/fo/Recipe
fo:Recipe rdf:type owl:Class .


###  http://purl.org/ontology/fo/Season
fo:Season rdf:type owl:Class ;
          rdfs:comment "A Season is a period of time that recurs annually during which a food is typically available or at its best."@en-gb ;
          rdfs:isDefinedBy fo: ;
          rdfs:label "Season"@en-gb ;
          vs:term_status "testing" .


###  http://purl.org/ontology/fo/StageSequence
fo:StageSequence rdf:type owl:Class ;
                 rdfs:subClassOf rdf:Seq ;
                 rdfs:comment "Where a recipe has a number of stage, for example where a recipe states 'for the sauce' a stage sequence provides a way to sequence the stages (rdf:Seq) into the desired order."@en-gb ;
                 rdfs:isDefinedBy fo: ;
                 rdfs:label "StageSequence"@en-gb ;
                 vs:term_status "testing" .


###  http://purl.org/ontology/fo/Technique
fo:Technique rdf:type owl:Class ;
             rdfs:comment "A Technique is a way of working with an ingredient to produce a desired effect, for example, whipping cream."@en-gb ;
             rdfs:isDefinedBy fo: ;
             rdfs:label "Technique"@en-gb ;
             vs:term_status "testing" .


###  http://www.w3.org/1999/02/22-rdf-syntax-ns#Seq
rdf:Seq rdf:type owl:Class .


#################################################################
#    Individuals
#################################################################

###  http://creativecommons.org/licenses/by/4.0#id
<http://creativecommons.org/licenses/by/4.0#id> rdf:type owl:NamedIndividual .


###  http://purl.org/dc/aboutdcmi#DCMI
<http://purl.org/dc/aboutdcmi#DCMI> rdf:type owl:NamedIndividual .


###  http://purl.org/ontology/fo/
fo: rdf:type owl:NamedIndividual .


###  http://purl.org/ontology/fo/Ingredient
fo:Ingredient rdf:type owl:NamedIndividual ;
              owl:sameAs v:Ingredient .


###  http://purl.org/ontology/fo/Recipe
fo:Recipe rdf:type owl:NamedIndividual ;
          owl:sameAs v:Recipe .


###  http://purl.org/ontology/fo/#andrew
<http://purl.org/ontology/fo/#andrew> rdf:type owl:NamedIndividual .


###  http://purl.org/ontology/fo/#oliver
<http://purl.org/ontology/fo/#oliver> rdf:type owl:NamedIndividual .


###  http://purl.org/ontology/fo/#philip
<http://purl.org/ontology/fo/#philip> rdf:type owl:NamedIndividual .


###  http://purl.org/ontology/fo/#rija
<http://purl.org/ontology/fo/#rija> rdf:type owl:NamedIndividual .


###  http://purl.org/ontology/fo/#rob
<http://purl.org/ontology/fo/#rob> rdf:type owl:NamedIndividual .


###  http://rdf.data-vocabulary.org/#Ingredient
v:Ingredient rdf:type owl:NamedIndividual .


###  http://rdf.data-vocabulary.org/#Recipe
v:Recipe rdf:type owl:NamedIndividual .


#################################################################
#    Annotations
#################################################################

dc: dcterms:publisher <http://purl.org/dc/aboutdcmi#DCMI> ;
    dcterms:title "Dublin Core Metadata Element Set, Version 1.1"@en ;
    dcterms:modified "2012-06-14"^^xsd:date .


fo:Ingredient rdfs:comment "An Ingredient is the combination of a quantity and a food, giving the amount of something that should be used in the recipe."@en-gb ;
              rdfs:isDefinedBy fo: ;
              vs:term_status "testing" ;
              rdfs:label "Ingredient"@en-gb .


fo:Recipe vs:term_status "testing" ;
          rdfs:isDefinedBy fo: ;
          rdfs:label "Recipe"@en-gb ;
          rdfs:comment "A Recipe is a combination of ingredients and a method, created by a chef, that produces a food."@en-gb .


###  Generated by the OWL API (version 4.2.8.20170104-2310) https://github.com/owlcs/owlapi
