<?xml version="1.0"?>
<rdf:RDF xmlns="http://rdfs.org/sioc/ns#"
     xml:base="http://rdfs.org/sioc/ns"
     xmlns:rdf="http://www.w3.org/1999/02/22-rdf-syntax-ns#"
     xmlns:owl="http://www.w3.org/2002/07/owl#"
     xmlns:xml="http://www.w3.org/XML/1998/namespace"
     xmlns:xsd="http://www.w3.org/2001/XMLSchema#"
     xmlns:dcterms="http://purl.org/dc/terms/"
     xmlns:rdfs="http://www.w3.org/2000/01/rdf-schema#"
     xmlns:vs="http://www.w3.org/2003/06/sw-vocab-status/ns#"
     xmlns:wot="http://xmlns.com/wot/0.1/"
     xmlns:foaf="http://xmlns.com/foaf/0.1/"
     xmlns:sioc="http://rdfs.org/sioc/ns#">
    <owl:Ontology rdf:about="http://rdfs.org/sioc/ns#">
        <owl:versionInfo>Revision: 1.36</owl:versionInfo>
        <rdfs:seeAlso rdf:resource="http://rdfs.org/sioc/spec"/>
    </owl:Ontology>
    


    <!-- 
    ///////////////////////////////////////////////////////////////////////////////////////
    //
    // Data properties
    //
    ///////////////////////////////////////////////////////////////////////////////////////
     -->

    


    <!-- http://purl.org/dc/terms/date -->

    <owl:DatatypeProperty rdf:about="http://purl.org/dc/terms/date"/>
    


    <!-- http://purl.org/dc/terms/description -->

    <owl:DatatypeProperty rdf:about="http://purl.org/dc/terms/description"/>
    


    <!-- http://purl.org/dc/terms/title -->

    <owl:DatatypeProperty rdf:about="http://purl.org/dc/terms/title"/>
    


    <!-- http://rdfs.org/sioc/ns#content -->

    <owl:DatatypeProperty rdf:about="http://rdfs.org/sioc/ns#content">
        <rdfs:range rdf:resource="http://www.w3.org/2000/01/rdf-schema#Literal"/>
        <rdfs:comment xml:lang="en">The content of the Item in plain text format.</rdfs:comment>
        <rdfs:isDefinedBy rdf:resource="http://rdfs.org/sioc/ns#"/>
        <rdfs:label xml:lang="en">content</rdfs:label>
    </owl:DatatypeProperty>
    


    <!-- http://rdfs.org/sioc/ns#last_activity_date -->

    <owl:DatatypeProperty rdf:about="http://rdfs.org/sioc/ns#last_activity_date">
        <rdfs:subPropertyOf rdf:resource="http://purl.org/dc/terms/date"/>
        <rdfs:range rdf:resource="http://www.w3.org/2000/01/rdf-schema#Literal"/>
        <rdfs:comment xml:lang="en">The date and time of the last activity associated with a SIOC concept instance, and expressed in ISO 8601 format. This could be due to a reply Post or Comment, a modification to an Item, etc.</rdfs:comment>
        <rdfs:isDefinedBy rdf:resource="http://rdfs.org/sioc/ns#"/>
        <rdfs:label xml:lang="en">last activity date</rdfs:label>
    </owl:DatatypeProperty>
    


    <!-- http://rdfs.org/sioc/ns#last_item_date -->

    <owl:DatatypeProperty rdf:about="http://rdfs.org/sioc/ns#last_item_date">
        <rdfs:subPropertyOf rdf:resource="http://purl.org/dc/terms/date"/>
        <rdfs:range rdf:resource="http://www.w3.org/2000/01/rdf-schema#Literal"/>
        <rdfs:comment xml:lang="en">The date and time of the last Post (or Item) in a Forum (or a Container), in ISO 8601 format.</rdfs:comment>
        <rdfs:isDefinedBy rdf:resource="http://rdfs.org/sioc/ns#"/>
        <rdfs:label xml:lang="en">last item date</rdfs:label>
    </owl:DatatypeProperty>
    


    <!-- http://rdfs.org/sioc/ns#last_reply_date -->

    <owl:DatatypeProperty rdf:about="http://rdfs.org/sioc/ns#last_reply_date">
        <rdfs:subPropertyOf rdf:resource="http://purl.org/dc/terms/date"/>
        <rdfs:range rdf:resource="http://www.w3.org/2000/01/rdf-schema#Literal"/>
        <rdfs:comment xml:lang="en">The date and time of the last reply Post or Comment, which could be associated with a starter Item or Post or with a Thread, and expressed in ISO 8601 format.</rdfs:comment>
        <rdfs:isDefinedBy rdf:resource="http://rdfs.org/sioc/ns#"/>
        <rdfs:label xml:lang="en">last reply date</rdfs:label>
    </owl:DatatypeProperty>
    


    <!-- 
    ///////////////////////////////////////////////////////////////////////////////////////
    //
    // Individuals
    //
    ///////////////////////////////////////////////////////////////////////////////////////
     -->

    


    <!-- http://rdfs.org/sioc/ns# -->

    <owl:Thing rdf:about="http://rdfs.org/sioc/ns#">
        <rdf:type rdf:resource="http://www.w3.org/2002/07/owl#NamedIndividual"/>
        <dcterms:description xml:lang="en">SIOC (Semantically-Interlinked Online Communities) is an ontology for describing the information in online communities. 
This information can be used to export information from online communities and to link them together. The scope of the application areas that SIOC can be used for includes (and is not limited to) weblogs, message boards, mailing lists and chat channels.</dcterms:description>
        <dcterms:title xml:lang="en">SIOC Core Ontology Namespace</dcterms:title>
    </owl:Thing>
    


    <!-- 
    ///////////////////////////////////////////////////////////////////////////////////////
    //
    // Annotations
    //
    ///////////////////////////////////////////////////////////////////////////////////////
     -->

    <rdf:Description rdf:about="http://rdfs.org/sioc/spec">
        <rdfs:label>SIOC Core Ontology Specification</rdfs:label>
    </rdf:Description>
</rdf:RDF>



<!-- Generated by the OWL API (version 4.2.8.20170104-2310) https://github.com/owlcs/owlapi -->

