<?xml version="1.0"?>
<rdf:RDF xmlns="http://socsem.open.ac.uk/ontologies/eu#"
     xml:base="http://socsem.open.ac.uk/ontologies/eu"
     xmlns:rdf="http://www.w3.org/1999/02/22-rdf-syntax-ns#"
     xmlns:terms="http://purl.org/dc/terms/"
     xmlns:owl="http://www.w3.org/2002/07/owl#"
     xmlns:ns="http://creativecommons.org/ns#"
     xmlns:muo="http://purl.oclc.org/NET/muo/muo#"
     xmlns:xml="http://www.w3.org/XML/1998/namespace"
     xmlns:xsd="http://www.w3.org/2001/XMLSchema#"
     xmlns:rdfs="http://www.w3.org/2000/01/rdf-schema#"
     xmlns:vann="http://purl.org/vocab/vann/"
     xmlns:foaf="http://xmlns.com/foaf/0.1/"
     xmlns:dc="http://purl.org/dc/elements/1.1/">
    <owl:Ontology rdf:about="http://socsem.open.ac.uk/ontologies/eu#">
        <owl:imports rdf:resource="http://elite.polito.it/ontologies/poweront.owl"/>
        <owl:imports rdf:resource="http://purl.org/muto/core"/>
        <dc:date>2016-04-22</dc:date>
        <rdfs:seeAlso rdf:resource="http://energyuse.eu"/>
        <dc:description rdf:resource="http://socsem.open.ac.uk/ontologies/eu.png"/>
        <rdfs:comment xml:lang="en">The EnergyUse ontology is a model for representing the public content of the energyuse.eu website. In particular, it allows the publication of discussions related to energy consumption and the modelling of actual aggregated energy consumption measures of home appliances.

This document represents the Energy Use ontology definition of the most important entities and atributes required for publishing content similar to the one produced in the EnergyUse platform.</rdfs:comment>
        <terms:modified rdf:datatype="http://www.w3.org/2001/XMLSchema#date">2012-06-14</terms:modified>
        <dc:description xml:lang="en">The Energy Use ontology is a model for representing the public content of the energyuse.eu website. In particular, it allows the publication of discussions related to energy consumption and the modelling of actual aggregated energy consumption measures of home appliances.</dc:description>
        <dc:creator>Gr√©goire Burel</dc:creator>
        <dc:title rdf:datatype="http://www.w3.org/2001/XMLSchema#string">Energy Use Ontology</dc:title>
    </owl:Ontology>
    


    <!-- 
    ///////////////////////////////////////////////////////////////////////////////////////
    //
    // Object Properties
    //
    ///////////////////////////////////////////////////////////////////////////////////////
     -->

    


    <!-- http://socsem.open.ac.uk/ontologies/eu#concept -->

    <owl:ObjectProperty rdf:about="http://socsem.open.ac.uk/ontologies/eu#concept">
        <rdfs:comment xml:lang="en">A Concept linked to a discussion.</rdfs:comment>
        <rdfs:label>concept</rdfs:label>
    </owl:ObjectProperty>
    


    <!-- http://socsem.open.ac.uk/ontologies/eu#consumptionSummary -->

    <owl:ObjectProperty rdf:about="http://socsem.open.ac.uk/ontologies/eu#consumptionSummary">
        <rdfs:range rdf:resource="http://socsem.open.ac.uk/ontologies/eu#ElectricEnergyConsumptionSummary"/>
        <rdfs:comment xml:lang="en">Link summary statistics about the consumption of a given appliance.</rdfs:comment>
        <rdfs:label>consumptionSummary</rdfs:label>
    </owl:ObjectProperty>
    


    <!-- http://socsem.open.ac.uk/ontologies/eu#meaning -->

    <owl:ObjectProperty rdf:about="http://socsem.open.ac.uk/ontologies/eu#meaning">
        <rdfs:comment xml:lang="en">Connect a given Concept with a particular entity that define the given concept (e.g. DBPedia resource).</rdfs:comment>
        <rdfs:label>meaning</rdfs:label>
    </owl:ObjectProperty>
    


    <!-- http://socsem.open.ac.uk/ontologies/eu#measure -->

    <owl:ObjectProperty rdf:about="http://socsem.open.ac.uk/ontologies/eu#measure">
        <rdfs:domain rdf:resource="http://socsem.open.ac.uk/ontologies/eu#SummaryStatistic"/>
        <rdfs:comment xml:lang="en">Define the Measure used for a given SUmmaryStatistic.</rdfs:comment>
        <rdfs:label>measure</rdfs:label>
    </owl:ObjectProperty>
    


    <!-- http://socsem.open.ac.uk/ontologies/eu#statistic -->

    <owl:ObjectProperty rdf:about="http://socsem.open.ac.uk/ontologies/eu#statistic">
        <rdfs:domain rdf:resource="http://socsem.open.ac.uk/ontologies/eu#DataSummary"/>
        <rdfs:range rdf:resource="http://socsem.open.ac.uk/ontologies/eu#SummaryStatistic"/>
        <rdfs:comment xml:lang="en">Associate a SummaryStatistic with a DataSummary.</rdfs:comment>
        <rdfs:label>statistic</rdfs:label>
    </owl:ObjectProperty>
    


    <!-- 
    ///////////////////////////////////////////////////////////////////////////////////////
    //
    // Data properties
    //
    ///////////////////////////////////////////////////////////////////////////////////////
     -->

    


    <!-- http://purl.org/dc/terms/description -->

    <owl:DatatypeProperty rdf:about="http://purl.org/dc/terms/description">
        <owl:equivalentProperty rdf:resource="http://socsem.open.ac.uk/ontologies/eu#description"/>
    </owl:DatatypeProperty>
    


    <!-- http://rdfs.org/sioc/ns#content -->

    <owl:DatatypeProperty rdf:about="http://rdfs.org/sioc/ns#content">
        <owl:equivalentProperty rdf:resource="http://socsem.open.ac.uk/ontologies/eu#content"/>
    </owl:DatatypeProperty>
    


    <!-- http://socsem.open.ac.uk/ontologies/eu#content -->

    <owl:DatatypeProperty rdf:about="http://socsem.open.ac.uk/ontologies/eu#content">
        <rdfs:range rdf:resource="http://www.w3.org/2000/01/rdf-schema#Literal"/>
        <rdfs:comment xml:lang="en">Represents the content assossiated witha given Post.</rdfs:comment>
        <rdfs:label>content</rdfs:label>
    </owl:DatatypeProperty>
    


    <!-- http://socsem.open.ac.uk/ontologies/eu#created -->

    <owl:DatatypeProperty rdf:about="http://socsem.open.ac.uk/ontologies/eu#created">
        <rdfs:range rdf:resource="http://www.w3.org/2001/XMLSchema#dateTimeStamp"/>
        <rdfs:comment xml:lang="en">A timestamp representing when a particular Post was created.</rdfs:comment>
        <rdfs:label>created</rdfs:label>
    </owl:DatatypeProperty>
    


    <!-- http://socsem.open.ac.uk/ontologies/eu#description -->

    <owl:DatatypeProperty rdf:about="http://socsem.open.ac.uk/ontologies/eu#description">
        <rdfs:range rdf:resource="http://www.w3.org/2000/01/rdf-schema#Literal"/>
        <rdfs:comment xml:lang="en">A textual description of a given Concept.</rdfs:comment>
        <rdfs:label>description</rdfs:label>
    </owl:DatatypeProperty>
    


    <!-- http://socsem.open.ac.uk/ontologies/eu#energyValue -->

    <owl:DatatypeProperty rdf:about="http://socsem.open.ac.uk/ontologies/eu#energyValue">
        <rdfs:domain rdf:resource="http://socsem.open.ac.uk/ontologies/eu#ElectricEnergyConsumptionSummary"/>
        <rdfs:range rdf:resource="http://www.w3.org/2001/XMLSchema#double"/>
        <rdfs:comment xml:lang="en">The numerical value associated with a given ElectricEnergyStatistic statistic.</rdfs:comment>
        <rdfs:label>energyValue</rdfs:label>
    </owl:DatatypeProperty>
    


    <!-- http://socsem.open.ac.uk/ontologies/eu#label -->

    <owl:DatatypeProperty rdf:about="http://socsem.open.ac.uk/ontologies/eu#label">
        <rdfs:range rdf:resource="http://www.w3.org/2000/01/rdf-schema#Literal"/>
        <rdfs:comment xml:lang="en">A label decribing a given tag.</rdfs:comment>
        <rdfs:label>label</rdfs:label>
    </owl:DatatypeProperty>
    


    <!-- http://socsem.open.ac.uk/ontologies/eu#username -->

    <owl:DatatypeProperty rdf:about="http://socsem.open.ac.uk/ontologies/eu#username">
        <rdfs:range rdf:resource="http://www.w3.org/2000/01/rdf-schema#Literal"/>
        <rdfs:comment xml:lang="en">A username used for representing a user in a given platform.</rdfs:comment>
        <rdfs:label>username</rdfs:label>
    </owl:DatatypeProperty>
    


    <!-- 
    ///////////////////////////////////////////////////////////////////////////////////////
    //
    // Classes
    //
    ///////////////////////////////////////////////////////////////////////////////////////
     -->

    


    <!-- http://socsem.open.ac.uk/ontologies/eu#DataSummary -->

    <owl:Class rdf:about="http://socsem.open.ac.uk/ontologies/eu#DataSummary">
        <rdfs:comment xml:lang="en">A DataSummary represents high level information about a data distribution in terms of information providers and number of observations.</rdfs:comment>
        <rdfs:label>DataSummary</rdfs:label>
    </owl:Class>
    


    <!-- http://socsem.open.ac.uk/ontologies/eu#ElectricEnergyConsumptionSummary -->

    <owl:Class rdf:about="http://socsem.open.ac.uk/ontologies/eu#ElectricEnergyConsumptionSummary">
        <rdfs:subClassOf rdf:resource="http://socsem.open.ac.uk/ontologies/eu#DataSummary"/>
        <rdfs:comment xml:lang="en">An ElectricEnergyConsumptionSummary represent the sumary of an energy consumption dataset.</rdfs:comment>
        <rdfs:label>ElectricEnergyConsumptionSummary</rdfs:label>
    </owl:Class>
    


    <!-- http://socsem.open.ac.uk/ontologies/eu#ElectricEnergyStatistic -->

    <owl:Class rdf:about="http://socsem.open.ac.uk/ontologies/eu#ElectricEnergyStatistic">
        <rdfs:subClassOf rdf:resource="http://socsem.open.ac.uk/ontologies/eu#SummaryStatistic"/>
    </owl:Class>
    


    <!-- http://socsem.open.ac.uk/ontologies/eu#SummaryStatistic -->

    <owl:Class rdf:about="http://socsem.open.ac.uk/ontologies/eu#SummaryStatistic">
        <rdfs:subClassOf rdf:resource="http://purl.oclc.org/NET/muo/muo#QualityValue"/>
        <rdfs:comment xml:lang="en">A summary statistic provides a praticular value for a given DataSummary. It is associated with a given Measure that defines the nature of the statistic.</rdfs:comment>
        <rdfs:label>SummaryStatistic</rdfs:label>
    </owl:Class>
    


    <!-- 
    ///////////////////////////////////////////////////////////////////////////////////////
    //
    // Individuals
    //
    ///////////////////////////////////////////////////////////////////////////////////////
     -->

    


    <!-- http://socsem.open.ac.uk/ontologies/eu#ElectricEnergyStatistic -->

    <owl:NamedIndividual rdf:about="http://socsem.open.ac.uk/ontologies/eu#ElectricEnergyStatistic">
        <rdf:type rdf:resource="http://socsem.open.ac.uk/ontologies/eu#ElectricEnergyStatistic"/>
        <muo:measuredIn rdf:resource="http://socsem.open.ac.uk/ontologies/eu#watt-hour"/>
    </owl:NamedIndividual>
    


    <!-- http://socsem.open.ac.uk/ontologies/eu#day-mean -->

    <owl:NamedIndividual rdf:about="http://socsem.open.ac.uk/ontologies/eu#day-mean">
        <rdfs:comment xml:lang="en">The mean value in a dataset aggreagted over days.</rdfs:comment>
        <rdfs:label>day-mean</rdfs:label>
    </owl:NamedIndividual>
    


    <!-- http://socsem.open.ac.uk/ontologies/eu#max -->

    <owl:NamedIndividual rdf:about="http://socsem.open.ac.uk/ontologies/eu#max">
        <rdfs:comment xml:lang="en">The maximum value in a dataset.</rdfs:comment>
        <rdfs:label>max</rdfs:label>
    </owl:NamedIndividual>
    


    <!-- http://socsem.open.ac.uk/ontologies/eu#mean -->

    <owl:NamedIndividual rdf:about="http://socsem.open.ac.uk/ontologies/eu#mean">
        <rdfs:comment xml:lang="en">The mean value in a dataset.</rdfs:comment>
        <rdfs:label>mean</rdfs:label>
    </owl:NamedIndividual>
    


    <!-- http://socsem.open.ac.uk/ontologies/eu#min -->

    <owl:NamedIndividual rdf:about="http://socsem.open.ac.uk/ontologies/eu#min">
        <rdfs:comment xml:lang="en">The minimum value in a dataset.</rdfs:comment>
        <rdfs:label xml:lang="en">min</rdfs:label>
    </owl:NamedIndividual>
    


    <!-- http://socsem.open.ac.uk/ontologies/eu#range -->

    <owl:NamedIndividual rdf:about="http://socsem.open.ac.uk/ontologies/eu#range">
        <rdfs:comment xml:lang="en">The range of a dataset.</rdfs:comment>
        <rdfs:label>range</rdfs:label>
    </owl:NamedIndividual>
    


    <!-- http://socsem.open.ac.uk/ontologies/eu#std-dev -->

    <owl:NamedIndividual rdf:about="http://socsem.open.ac.uk/ontologies/eu#std-dev">
        <rdfs:comment xml:lang="en">The standard deviation.</rdfs:comment>
        <rdfs:label>std-dev</rdfs:label>
    </owl:NamedIndividual>
    


    <!-- http://socsem.open.ac.uk/ontologies/eu#watt-hour -->

    <owl:NamedIndividual rdf:about="http://socsem.open.ac.uk/ontologies/eu#watt-hour">
        <rdf:type rdf:resource="http://purl.oclc.org/NET/muo/muo#UnitOfMeasurement"/>
        <rdfs:comment xml:lang="en">The watt-hours energy consumption unit (Wh).</rdfs:comment>
        <rdfs:label xml:lang="en">watt-hour</rdfs:label>
    </owl:NamedIndividual>
    


    <!-- 
    ///////////////////////////////////////////////////////////////////////////////////////
    //
    // Annotations
    //
    ///////////////////////////////////////////////////////////////////////////////////////
     -->

    <rdf:Description rdf:about="http://socsem.open.ac.uk/ontologies/eu#ElectricEnergyStatistic">
        <rdfs:comment xml:lang="en">An ElectricEnergyStatistic, is a statistic designed to measure the energy consumption of electric aplliances.</rdfs:comment>
        <rdfs:label>ElectricEnergyStatistic</rdfs:label>
    </rdf:Description>
</rdf:RDF>



<!-- Generated by the OWL API (version 4.2.8.20170104-2310) https://github.com/owlcs/owlapi -->

